new/proof/fmt.v
@@ -1,10 +1,25 @@
 From New.generatedproof Require Import fmt.
 From New.proof Require Import proof_prelude.
 
-Section proof.
-Context  `{hG: heapGS Σ, !ffi_semantics _ _} `{!globalsGS Σ} {go_ctx : GoContext}.
+Section wps.
+Context `{hG: heapGS Σ, !ffi_semantics _ _}.
+Context {sem : go.Semantics} {package_sem : fmt.Assumptions}.
+Local Set Default Proof Using "All".
 
-#[global] Instance : IsPkgInit fmt := define_is_pkg_init True%I.
-#[global] Instance : GetIsPkgInitWf fmt := build_get_is_pkg_init_wf.
+#[global] Instance : IsPkgInit (iProp Σ) fmt := define_is_pkg_init True%I.
+#[global] Instance : GetIsPkgInitWf (iProp Σ) fmt := build_get_is_pkg_init_wf.
 
-End proof.
+Lemma wp_initialize' get_is_pkg_init :
+  get_is_pkg_init_prop fmt get_is_pkg_init →
+  {{{ own_initializing get_is_pkg_init }}}
+    fmt.initialize' #()
+  {{{ RET #(); own_initializing get_is_pkg_init ∗ is_pkg_init fmt }}}.
+Proof.
+  intros Hinit. wp_start as "Hown".
+  wp_apply (wp_package_init with "[$Hown] HΦ").
+  { destruct Hinit as (-> & ?); done. }
+  iIntros "Hown". wp_auto.
+  iEval (rewrite is_pkg_init_unfold /=). iFrame "∗#".
+Admitted.
+
+End wps.
