new/proof/sync_proof/cond.v
@@ -1,21 +1,22 @@
 From New.proof.sync_proof Require Import base mutex.
 Local Existing Instances tokG wg_totalG rw_ghost_varG rw_ghost_wlG rw_ghost_rwmutexG  wg_auth_inG.
 
-Unset Printing Projections.
+Local Unset Printing Projections.
 
-Section proof.
-Context `{heapGS Σ, !ffi_semantics _ _}.
-Context `{!globalsGS Σ} {go_ctx : GoContext}.
+Section wps.
+Context `{hG: heapGS Σ, !ffi_semantics _ _}.
+Context {sem : go.Semantics} {package_sem : sync.Assumptions}.
+Local Set Default Proof Using "All".
 Context `{!syncG Σ}.
 
 (** This means [c] is a condvar with underyling Locker at address [m]. *)
 Definition is_Cond (c : loc) (m : interface.t) : iProp Σ :=
   "#Hi" ∷ is_pkg_init sync ∗
-  "#Hc" ∷ c ↦s[sync.Cond :: "L"]□ m ∗
-  (* TODO: not accurate to assume it never changes, there should be an unknown
+  "#Hc" ∷ c.[sync.Cond.t, "L"] ↦□ m ∗
+  (* FIXME: not accurate to assume it never changes, there should be an unknown
   notifyList struct in an invariant *)
-  "#?" ∷ c ↦s[sync.Cond :: "notify"]□ default_val sync.notifyList.t ∗
-  "#?" ∷ c ↦s[sync.Cond :: "checker"]□ default_val sync.copyChecker.t
+  "#?" ∷ c.[sync.Cond.t, "notify"] ↦□ zero_val sync.notifyList.t ∗
+  "#?" ∷ c.[sync.Cond.t, "checker"] ↦□ zero_val sync.copyChecker.t
 .
 #[global] Opaque is_Cond.
 #[local] Transparent is_Cond.
@@ -33,19 +34,15 @@ Proof.
   wp_alloc c as "Hc".
   wp_pures.
   iApply "HΦ".
-
-  iDestruct (struct_fields_split with "Hc") as "Hl".
-  cbn [sync.Cond.L' sync.Cond.noCopy' sync.Cond.notify' sync.Cond.checker'].
-  iNamed "Hl".
-  iClear "HnoCopy". (* not used *)
-  iPersist "HL Hchecker".
-  iPersist "Hnotify".
+  iStructNamed "Hc". simpl.
+  iClear "noCopy". (* not used *)
+  iPersist "L checker notify".
   iFrame "#". done.
 Qed.
 
 Lemma wp_copyChecker__check c (c_v: sync.copyChecker.t) dq :
   {{{ is_pkg_init sync ∗ c ↦{dq} c_v }}}
-    c @ (ptrT.id sync.copyChecker.id) @ "check" #()
+    c @! (go.PointerType sync.copyChecker) @! "check" #()
   {{{ RET #(); c ↦{dq} c_v }}}.
 Proof.
   wp_start as "c".
@@ -57,8 +54,8 @@ Lemma wp_runtime_notifyListAdd l (l_v: sync.notifyList.t) dq :
   {{{ (x: w32), RET #x; l ↦{dq} l_v }}}.
 Proof.
   wp_start as "l".
-  wp_apply wp_ArbitraryInt as "%".
-  iApply "HΦ". by iFrame.
+  wp_apply wp_ArbitraryInt as "% _".
+  wp_end.
 Qed.
 
 Lemma wp_runtime_notifyListNotifyOne l (l_v: sync.notifyList.t) dq :
@@ -66,8 +63,7 @@ Lemma wp_runtime_notifyListNotifyOne l (l_v: sync.notifyList.t) dq :
    @! sync.runtime_notifyListNotifyOne #l
   {{{ RET #(); l ↦{dq} l_v }}}.
 Proof.
-  wp_start as "l".
-  iApply "HΦ". by iFrame.
+  wp_start as "l". wp_end.
 Qed.
 
 Lemma wp_runtime_notifyListNotifyAll l (l_v: sync.notifyList.t) dq :
@@ -75,8 +71,7 @@ Lemma wp_runtime_notifyListNotifyAll l (l_v: sync.notifyList.t) dq :
    @! sync.runtime_notifyListNotifyAll #l
   {{{ RET #(); l ↦{dq} l_v }}}.
 Proof.
-  wp_start as "l".
-  iApply "HΦ". by iFrame.
+  wp_start as "l". wp_end.
 Qed.
 
 Lemma wp_runtime_notifyListWait l (l_v: sync.notifyList.t) (t: w32) dq :
@@ -84,37 +79,35 @@ Lemma wp_runtime_notifyListWait l (l_v: sync.notifyList.t) (t: w32) dq :
    @! sync.runtime_notifyListWait #l #t
   {{{ RET #(); l ↦{dq} l_v }}}.
 Proof.
-  wp_start as "l".
-  iApply "HΦ". by iFrame.
+  wp_start as "l". wp_end.
 Qed.
 
 Theorem wp_Cond__Signal c lk :
   {{{ is_Cond c lk }}}
-    c @ (ptrT.id sync.Cond.id) @ "Signal" #()
+    c @! (go.PointerType sync.Cond) @! "Signal" #()
   {{{ RET #(); True }}}.
 Proof.
   wp_start as "[#Hdef @]".
   wp_auto.
   wp_apply (wp_copyChecker__check with "[$]") as "?".
   wp_apply (wp_runtime_notifyListNotifyOne with "[$]") as "_".
-  iApply "HΦ". done.
+  wp_end.
 Qed.
 
 Theorem wp_Cond__Broadcast c lk :
   {{{ is_Cond c lk }}}
-    c @ (ptrT.id sync.Cond.id) @ "Broadcast" #()
+    c @! (go.PointerType sync.Cond) @! "Broadcast" #()
   {{{ RET #(); True }}}.
 Proof.
-  wp_start as "H"; iNamed "H".
-  wp_method_call. wp_call. wp_auto.
+  wp_start as "H"; iNamed "H". wp_auto.
   wp_apply (wp_copyChecker__check with "[$]") as "?".
   wp_apply (wp_runtime_notifyListNotifyAll with "[$]") as "_".
-  iApply "HΦ". done.
+  wp_end.
 Qed.
 
 Theorem wp_Cond__Wait c m R :
   {{{ is_Cond c m ∗ is_Locker m R ∗ R }}}
-    c @ (ptrT.id sync.Cond.id) @ "Wait" #()
+    c @! (go.PointerType sync.Cond) @! "Wait" #()
   {{{ RET #(); R }}}.
 Proof.
   wp_start as "(@ & #Hlock & HR)". wp_auto.
@@ -124,7 +117,7 @@ Proof.
   wp_apply ("H_Unlock" with "[$HR]").
   wp_apply (wp_runtime_notifyListWait with "[$]") as "_".
   wp_apply ("H_Lock" with "[$]") as "HR".
-  iApply "HΦ". by iFrame.
+  wp_end.
 Qed.
 
-End proof.
+End wps.
